# ss
$$\frac{2s^3 + 5s^2 + 6s + 7}{(s-3)(s^2 + 2s + 2)}  $$
$$\frac{A}{s-3} + \frac{Bs + C}{s^2 + 2s + 2}$$
$$ Bs + C = \frac{2s^3 + 5s^2 + 6s + 7(s^2 + 2s + 2)}{(s-3)(s^2 + 2s + 2)} \quad \text{evaluado en} \quad s = -1 + i$$
$$ \frac{2(-1+i)^3 + 5(-1+i)^2 + 6(-1+i) + 7}{(-1+i)-3} = B(-1+i) + C$$ 
$$ \frac{5}{-4+i} = -B + Bi + C$$ 
$$ \frac{-20}{17} - \frac{6i}{17} = -B + Bi + C$$ 
$$ \frac{-20}{17} - \frac{6i}{17} = -B + Bi + C$$ 
$$ \frac{-6i}{17} = Bi$$ 
$$  B = \frac{-6}{17}$$ 
$$ \frac{-20}{17} = -B + C$$ 
$$ \frac{-20}{17} = \frac{6}{17} + C$$ 
$$  C = \frac{-14}{17}$$ 
$$\frac{2s^3 + 5s^2 + 6s + 7}{s^2 + 2s + 2} \quad \text{evaluado en} \quad s = 3 $$
$$A = \frac{2(3)^3 + 5(3)^2 + 6(3) + 7}{(3)^2 + 2(3) + 2}$$
$$A = \frac{124}{17}$$
$$\frac{\frac{124}{17}}{s-3} + \frac{-\frac{6}{17}s - \frac{14}{17}}{s^2 + 2s + 2}$$
# eh
$$\frac{6s^2 + 11s + 10}{(s+2)(s^2 - 4s + 4)} $$
$$\frac{A}{s-2} + \frac{B}{(s-2)^2} + \frac{C}{s+2}$$
$$A = \frac{6s^2 + 11s + 10}{(s+2)(s^2 - 4s + 4)} \quad \text{evaluado en} \quad s = 2$$
