# Transformada de laplace 
$$\\frac{2s+7}{s^2 - 4s - 45}\$$
$$\\frac{2s+7}{(s-9)(s+5)}\$$
$$\\frac{2s+7}{(s-9)(s+5)} = \frac{A}{s-9} + \frac{B}{s+5}\$$
$$\\ 2s + 7 = A(s + 5) + B(s - 9)\$$
$$\\ 2s + 7 = As + 5A + Bs - 9B$$
$$\\begin{cases} 
A + B = 2 \\
5A - 9B = 7
\end{cases}\
$$
$$\\ A = -B - 2\$$
$$\\ 5(-B - 2) - 9B = 7\$$
$$\\ -5B - 10 - 9B = 7\$$
$$\\ B= \frac{7+10}{4}\$$
$$\\ B = \frac{-17}{4}\$$
$$\\ A = -\left(\frac{-17}{4}\right) - 2\$$ 
$$\\ A = \frac{9}{4}\$$
$$\\frac{9}{4(s-9)} - \frac{17}{4(s+5)}\$$
# EJEMPLO 2
$$\\frac{4s - 2}{s^3 - s^2 - 2s}\$$
$$\\frac{4s - 2}{s(s^2 - s - 2s)}\$$
$$\\frac{4s - 2}{s(s - 2)(s + 1)}\$$
$$\\frac{A}{s} + \frac{B}{s - 2} + \frac{C}{s + 1}\$$
$$\ 4s - 2 = A(s - 2)(s + 1) + B(s)(s + 1) + C(s)(s - 2) \$$
$$\ 4s - 2 = A(s^2 - s - 2) + B(s^2 + s) + C(s^2 - 2s)\$$
$$\ 4s - 2 = As^2 - As - 2A + Bs^2 + Bs + Cs^2 - 2Cs\$$
$$\\begin{cases}
A + B + C = 0\\
-A + B - 2C = 4\\
-2A = -2
\end{cases}\$$
$$\ A = 1\$$
$$\ C = -1 - B\$$
$$\ -A + B - 2(-1 - B) = 4\$$
$$\ 1 + B + 2 + 2B = 4\$$
$$\ B = 1\$$
$$\ C = -2\$$
$$\\frac{1}{s} + \frac{1}{s - 2} - \frac{2}{s + 1}\$$

